thys/Registers/Misc.thy
@@ -74,7 +74,7 @@ lemma mat_of_rows_list_carrier[simp]:
 lemma apply_id_cblinfun[simp]: \<open>(*\<^sub>V) id_cblinfun = id\<close>
   by auto
 
-text \<open>Overriding \\<^theory>\<open>Complex_Bounded_Operators.Complex_Bounded_Linear_Function\<close>.\<^term>\<open>sandwich\<close>.
+text \<open>Overriding \<^theory>\<open>Complex_Bounded_Operators.Complex_Bounded_Linear_Function\<close>.\<^term>\<open>sandwich\<close>.
       The latter is the same function but defined as a \<^typ>\<open>(_,_) cblinfun\<close> which is less convenient for us.\<close>
 definition sandwich where \<open>sandwich a b = a o\<^sub>C\<^sub>L b o\<^sub>C\<^sub>L a*\<close>
 
@@ -82,6 +82,11 @@ lemma clinear_sandwich[simp]: \<open>clinear (sandwich a)\<close>
   apply (rule clinearI)
    apply (simp add: bounded_cbilinear.add_left bounded_cbilinear_cblinfun_compose bounded_cbilinear.add_right sandwich_def)
   by (simp add: sandwich_def)
+
+lemma bounded_clinear_sandwich[simp]: \<open>bounded_clinear (sandwich a)\<close>
+  apply (rule bounded_clinearI[where K=\<open>norm a * norm a\<close>])
+   apply (auto simp add: bounded_cbilinear.add_left bounded_cbilinear_cblinfun_compose bounded_cbilinear.add_right sandwich_def)
+  by (smt (verit, ccfv_SIG) mult.commute mult_right_mono norm_adj norm_cblinfun_compose norm_ge_zero ordered_field_class.sign_simps(32))
 
 lemma sandwich_id[simp]: \<open>sandwich id_cblinfun = id\<close>
   by (auto simp: sandwich_def)
